extraction: Further refactoring of QueryStructures.v

src/CertifiedExtraction/Extraction/Refactor/TupleToListW.v
@@ -1,37 +1,32 @@
-(* Require Import Fiat.Examples.QueryStructure.ProcessScheduler. *)
 Require Import Fiat.QueryStructure.Implementation.DataStructures.BagADT.QueryStructureImplementation.
-(* Require Import Fiat.Common.i3list. *)
 Require Import Fiat.ADT.Core.
 
-(* Require Import CertifiedExtraction.Core. *)
-
-(* Require Import Bedrock.Platform.Facade.examples.QsADTs. *)
 Require Import Bedrock.Platform.Facade.examples.TuplesF.
 Require Import CertifiedExtraction.Utils.
 Require Import Bedrock.Memory.
 
-Notation BedrockElement := (@TuplesF.IndexedElement (list W)).
-Notation BedrockBag := (@TuplesF.IndexedEnsemble (list W)).
+Require Import Refactor.Basics.
 
-Fixpoint MakeVectorOfW N : Vector.t Type N :=
-  match N with
-  | O => Vector.nil Type
-  | S x => Vector.cons Type W x (MakeVectorOfW x)
-  end.
-
-Definition MakeWordHeading (N: nat) :=
-  {| NumAttr := N;
-     AttrList := MakeVectorOfW N |}.
-
-Notation FiatTuple N := (@RawTuple (MakeWordHeading N)).
-Notation FiatElement N := (@IndexedEnsembles.IndexedElement (FiatTuple N)).
-Notation FiatBag N := (@IndexedEnsembles.IndexedEnsemble (FiatTuple N)).
+(** [TupleToListW] *)
 
 Fixpoint ilist2ToListW {N} {struct N} : ilist2.ilist2 (B := fun x => x) (MakeVectorOfW N) -> list W :=
   match N as N0 return (@ilist2.ilist2 Type (fun x : Type => x) N0 (MakeVectorOfW N0) -> list W) with
   | 0 => fun _ => nil
   | S x => fun il => ilist2.ilist2_hd il :: ilist2ToListW (ilist2.ilist2_tl il)
   end.
+
+Lemma ilist2ToListW_inj :
+  forall n el el',
+    ilist2ToListW (N := n) el = ilist2ToListW el'
+    -> el = el'.
+Proof.
+  induction n; simpl; eauto.
+  - destruct el; destruct el'; reflexivity.
+  - destruct el; destruct el'; simpl; intros.
+    unfold ilist2.ilist2_tl, ilist2.ilist2_hd in *; simpl in *.
+    injections; f_equal.
+    eapply IHn; eassumption.
+Qed.
 
 Definition TupleToListW {N} (tuple: @RawTuple (MakeWordHeading N)) :=
   ilist2ToListW tuple.
@@ -46,30 +41,9 @@ Fixpoint ListWToilist2 (l : list W) : ilist2.ilist2 (B := fun x => x) (MakeVecto
   | x :: x0 => ilist2.icons2 x (ListWToilist2 x0)
   end.
 
-Definition ListWToTuple (l: list W) : @RawTuple (MakeWordHeading (List.length l)) :=
-  ListWToilist2 l.
-
-Definition IndexedElement_ListWToTuple (element: @IndexedElement (list W)) : FiatElement (List.length (indexedElement element)) :=
-  {| IndexedEnsembles.elementIndex := element.(elementIndex);
-     IndexedEnsembles.indexedElement := ListWToTuple element.(indexedElement) |}.
-
-Lemma IndexedElement_RoundTrip :
-  forall l, IndexedElement_TupleToListW (IndexedElement_ListWToTuple l) = l.
-Proof.
-  destruct l.
-  induction indexedElement; simpl.
-  - reflexivity.
-  - unfold IndexedElement_ListWToTuple, IndexedElement_TupleToListW in *. simpl in *.
-    f_equal. inversion IHindexedElement. rewrite H0. unfold TupleToListW in *.
-    simpl. f_equal. compute in *. rewrite H0. reflexivity.
-Qed.
-
 Definition RelatedIndexedTupleAndListW {N} (l: BedrockElement) (tup: FiatElement N) :=
   l.(elementIndex) = tup.(IndexedEnsembles.elementIndex) /\
   l.(indexedElement) = TupleToListW tup.(IndexedEnsembles.indexedElement).
-
-Definition IndexedEnsemble_TupleToListW {N} (ensemble: FiatBag N) : BedrockBag :=
-  fun listW => exists tup, ensemble tup /\ RelatedIndexedTupleAndListW listW tup.
 
 Lemma TupleToListW_inj {N}:
   forall (t1 t2: @RawTuple (MakeWordHeading N)),
@@ -95,12 +69,6 @@ Qed.
 
 Hint Resolve map_TupleToListW_inj : inj_db.
 
-Lemma lift_eq {A} (f g: A -> Prop) :
-  f = g -> (forall x, f x <-> g x).
-Proof.
-  intros; subst; reflexivity.
-Qed.
-
 Lemma IndexedElement_TupleToListW_inj :
   forall {N} (e1 e2: FiatElement N),
     IndexedElement_TupleToListW e1 = IndexedElement_TupleToListW e2 ->
@@ -110,36 +78,69 @@ Proof.
   apply TupleToListW_inj; eauto.
 Qed.
 
-Lemma IndexedEnsemble_TupleToListW_inj_helper:
-  forall (N : nat) (e : FiatBag N) (x : FiatElement N),
-    (IndexedEnsemble_TupleToListW e (IndexedElement_TupleToListW (N := N) x)) <-> e x.
+
+Lemma TupleToListW_length:
+  forall (N : nat) (tuple : FiatTuple N),
+    BinNat.N.lt (BinNat.N.of_nat N) (Word.Npow2 32) ->
+    Datatypes.length (TupleToListW tuple) = Word.wordToNat (Word.natToWord 32 N).
 Proof.
-  unfold IndexedEnsemble_TupleToListW, RelatedIndexedTupleAndListW;
-  repeat match goal with
-         | _ => cleanup
-         | _ => eassumption
-         | _ => progress subst
-         | [ x: FiatElement _ |- _ ] => destruct x
-         | [ H: TupleToListW _ = TupleToListW _ |- _ ] => apply TupleToListW_inj in H
-         | _ => eexists
-         | _ => simpl in *
-         end.
+  intros; rewrite Word.wordToNat_natToWord_idempotent by assumption.
+  clear H.
+  induction N; intros.
+  - destruct tuple; reflexivity.
+  - simpl; f_equal; apply IHN.
 Qed.
 
-Lemma IndexedEnsemble_TupleToListW_inj :
-  forall {N} (e1 e2: FiatBag N),
-    IndexedEnsemble_TupleToListW e1 = IndexedEnsemble_TupleToListW e2 ->
-    e1 = e2.
+Lemma TupleToListW_length':
+  forall (N : nat) (tuple : FiatTuple N),
+    BinNat.N.lt (BinNat.N.of_nat N) (Word.Npow2 32) ->
+    Datatypes.length (TupleToListW tuple) = N.
 Proof.
-  intros * H; pose proof (lift_eq H); clear H.
-  apply Ensembles.Extensionality_Ensembles; unfold Ensembles.Same_set, Ensembles.Included, Ensembles.In.
-  repeat cleanup; repeat match goal with
-                         | [ H: forall _, _ |- _ ?x ] => specialize (H (IndexedElement_TupleToListW x)); cbv beta in H
-                         | [ H: _ |- _ ] => setoid_rewrite IndexedEnsemble_TupleToListW_inj_helper in H
-                         end; tauto.
+  cleanup;
+  erewrite <- Word.wordToNat_natToWord_idempotent;
+  eauto using TupleToListW_length.
 Qed.
 
-Hint Resolve IndexedEnsemble_TupleToListW_inj : inj_db.
+Definition TupleToListW_indexed {N} (tup: FiatElement N) :=
+  {| TuplesF.elementIndex := IndexedEnsembles.elementIndex tup;
+     TuplesF.indexedElement := (TupleToListW (IndexedEnsembles.indexedElement tup)) |}.
+
+Lemma RelatedIndexedTupleAndListW_refl :
+  forall {N} tup,
+    @RelatedIndexedTupleAndListW N (TupleToListW_indexed tup) tup.
+Proof.
+  cleanup; red; intuition.
+Qed.
+
+Lemma TupleToListW_indexed_inj {N}:
+  forall (t1 t2: FiatElement N),
+    TupleToListW_indexed t1 = TupleToListW_indexed t2 ->
+    t1 = t2.
+Proof.
+  destruct t1, t2; unfold TupleToListW_indexed; simpl.
+  intro eq; inversion eq; subst; clear eq.
+  f_equal; intuition.
+Qed.
+
+(** [ListWToTuple] *)
+
+Definition ListWToTuple (l: list W) : @RawTuple (MakeWordHeading (List.length l)) :=
+  ListWToilist2 l.
+
+Definition IndexedElement_ListWToTuple (element: @IndexedElement (list W)) : FiatElement (List.length (indexedElement element)) :=
+  {| IndexedEnsembles.elementIndex := element.(elementIndex);
+     IndexedEnsembles.indexedElement := ListWToTuple element.(indexedElement) |}.
+
+Lemma IndexedElement_RoundTrip :
+  forall l, IndexedElement_TupleToListW (IndexedElement_ListWToTuple l) = l.
+Proof.
+  destruct l.
+  induction indexedElement; simpl.
+  - reflexivity.
+  - unfold IndexedElement_ListWToTuple, IndexedElement_TupleToListW in *. simpl in *.
+    f_equal. inversion IHindexedElement. rewrite H0. unfold TupleToListW in *.
+    simpl. f_equal. compute in *. rewrite H0. reflexivity.
+Qed.
 
 Fixpoint TruncateList {A} (a: A) n l :=
   match n, l with
@@ -187,39 +188,5 @@ Proof.
   destruct (TruncateList_length (Datatypes.length l) (Word.natToWord 32 0) l).
   rewrite IHl at 1.
   reflexivity.
-Qed.
-
-Definition FiatEmpty N : FiatBag N := fun _ => False.
-
-Lemma Empty_lift:
-  forall N : nat,
-    Empty = IndexedEnsemble_TupleToListW (FiatEmpty N).
-Proof.
-  intros; apply Ensembles.Extensionality_Ensembles.
-  unfold Ensembles.Same_set, Ensembles.Included, Ensembles.In, FiatEmpty, Empty, IndexedEnsemble_TupleToListW; split; intros.
-  - exfalso; assumption.
-  - repeat cleanup.
-Qed.
-
-Lemma TupleToListW_length:
-  forall (N : nat) (tuple : FiatTuple N),
-    BinNat.N.lt (BinNat.N.of_nat N) (Word.Npow2 32) ->
-    Datatypes.length (TupleToListW tuple) = Word.wordToNat (Word.natToWord 32 N).
-Proof.
-  intros; rewrite Word.wordToNat_natToWord_idempotent by assumption.
-  clear H.
-  induction N; intros.
-  - destruct tuple; reflexivity.
-  - simpl; f_equal; apply IHN.
-Qed.
-
-Lemma TupleToListW_length':
-  forall (N : nat) (tuple : FiatTuple N),
-    BinNat.N.lt (BinNat.N.of_nat N) (Word.Npow2 32) ->
-    Datatypes.length (TupleToListW tuple) = N.
-Proof.
-  cleanup;
-  erewrite <- Word.wordToNat_natToWord_idempotent;
-  eauto using TupleToListW_length.
 Qed.
 
