src/CertifiedExtraction/Benchmarks/QueryStructureWrappers.v
@@ -11,7 +11,10 @@ Require Import Bedrock.Platform.Facade.examples.TuplesF.
 Require Import CertifiedExtraction.Utils.
 
 Require Import Bedrock.Memory.
+
+Require Import Refactor.Basics.
 Require Import Refactor.TupleToListW.
+Require Import Refactor.EnsemblesOfTuplesAndListW.
 
 Ltac Wrapper_t :=
   abstract (intros * H; inversion H; subst; clear H; f_equal;
@@ -35,6 +38,11 @@ Proof.
             wrap_inj := _ |}; Wrapper_t.
 Defined.
 
+Instance QS_WrapBedrockTuple : FacadeWrapper QsADTs.ADTValue (TuplesF.tupl).
+Proof.
+  refine {| wrap tp := QsADTs.Tuple tp;
+            wrap_inj := _ |}; Wrapper_t.
+Defined.
 
 Instance QS_WrapBag0 {N} : FacadeWrapper ADTValue (FiatBag N).
 Proof.
@@ -53,215 +61,3 @@ Proof.
   refine {| wrap tl := Tuples2 (Word.natToWord 32 N) M M' (IndexedEnsemble_TupleToListW tl);
             wrap_inj := _ |}; Wrapper_t.
 Defined.
-
-Require Import CertifiedExtraction.Extraction.External.Core.
-Require Import Bedrock.Platform.Facade.examples.QsADTs.
-
-Section TupleLists.
-  Lemma CompileTupleList_new :
-    forall vret fpointer (env: Env ADTValue) ext tenv N,
-      GLabelMap.find fpointer env = Some (Axiomatic TupleList_new) ->
-      vret ∉ ext ->
-      Lifted_not_mapsto_adt ext tenv vret ->
-      {{ tenv }}
-        Call vret fpointer nil
-      {{ [[ `vret <-- @nil (FiatTuple N) as _ ]] :: DropName vret tenv }} ∪ {{ ext }} // env.
-  Proof.
-    repeat (SameValues_Facade_t_step || facade_cleanup_call || LiftPropertyToTelescope_t).
-    change (ADT (TupleList [])) with (wrap (FacadeWrapper := WrapInstance (H := @QS_WrapTupleList N)) []).
-    facade_eauto.
-  Qed.
-
-  Lemma CompileTupleList_delete :
-    forall vret vlst fpointer (env: Env ADTValue) ext tenv N,
-      GLabelMap.find fpointer env = Some (Axiomatic TupleList_delete) ->
-      Lifted_MapsTo ext tenv vlst (wrap (@nil (FiatTuple N))) ->
-      Lifted_not_mapsto_adt ext tenv vret ->
-      vret <> vlst ->
-      vlst ∉ ext ->
-      vret ∉ ext ->
-      {{ tenv }}
-        Call vret fpointer (vlst :: nil)
-      {{ [[ `vret <-- SCAZero as _ ]] :: DropName vret (DropName vlst tenv) }} ∪ {{ ext }} // env.
-  Proof.
-    repeat (SameValues_Facade_t_step || facade_cleanup_call || LiftPropertyToTelescope_t).
-    facade_eauto.
-    facade_eauto.
-  Qed.
-
-  Lemma CompileTupleList_pop :
-    forall vret vlst fpointer (env: Env ADTValue) ext tenv N
-      h (t: list (FiatTuple N)),
-      GLabelMap.find fpointer env = Some (Axiomatic TupleList_pop) ->
-      Lifted_MapsTo ext tenv vlst (wrap (h :: t)) ->
-      Lifted_not_mapsto_adt ext tenv vret ->
-      vret <> vlst ->
-      vlst ∉ ext ->
-      vret ∉ ext ->
-      {{ tenv }}
-        Call vret fpointer (vlst :: nil)
-        {{ [[ `vret <-- h as _ ]] :: [[ `vlst <-- t as _ ]] :: DropName vlst (DropName vret tenv) }} ∪ {{ ext }} // env.
-  Proof.
-    repeat (SameValues_Facade_t_step || facade_cleanup_call || LiftPropertyToTelescope_t).
-    facade_eauto.
-    facade_eauto.
-    facade_eauto.
-  Qed.
-
-  Lemma CompileTupleList_push :
-    forall vret vhd vlst fpointer (env: Env ADTValue) ext tenv N
-      h (t: list (FiatTuple N)),
-      GLabelMap.find fpointer env = Some (Axiomatic TupleList_push) ->
-      Lifted_MapsTo ext tenv vhd (wrap h) ->
-      Lifted_MapsTo ext tenv vlst (wrap t) ->
-      Lifted_not_mapsto_adt ext tenv vret ->
-      vret <> vlst ->
-      vret <> vhd ->
-      vhd <> vlst ->
-      vhd ∉ ext ->
-      vlst ∉ ext ->
-      vret ∉ ext ->
-      {{ tenv }}
-        Call vret fpointer (vlst :: vhd :: nil)
-        {{ [[ `vret <-- SCAZero as _ ]] :: [[ `vlst <-- h :: t as _ ]] :: DropName vlst (DropName vret (DropName vhd tenv)) }} ∪ {{ ext }} // env.
-  Proof.
-    repeat (SameValues_Facade_t_step || facade_cleanup_call || LiftPropertyToTelescope_t).
-    facade_eauto.
-    facade_eauto.
-    facade_eauto.
-    repeat apply DropName_remove; congruence.
-  Qed.
-End TupleLists.
-
-Hint Resolve Empty_lift : call_helpers_db.
-Hint Resolve TupleToListW_length : call_helpers_db.
-
-Section Tuples0.
-  Lemma CompileTuples0_new :
-    forall vret vsize fpointer (env: Env ADTValue) ext tenv N,
-      GLabelMap.find fpointer env = Some (Axiomatic Tuples0_new) ->
-      Lifted_MapsTo ext tenv vsize (wrap (Word.natToWord 32 N)) ->
-      Lifted_not_mapsto_adt ext tenv vret ->
-      vret ∉ ext ->
-      ~ Word.wlt (Word.natToWord 32 N) (Word.natToWord 32 2) ->
-      {{ tenv }}
-        Call vret fpointer (vsize :: nil)
-      {{ [[ `vret <-- @FiatEmpty N as _ ]] :: DropName vret tenv }} ∪ {{ ext }} // env.
-  Proof.
-    repeat (SameValues_Facade_t_step || facade_cleanup_call || LiftPropertyToTelescope_t).
-    facade_eauto.
-    repeat f_equal; facade_eauto.
-    facade_eauto.
-  Qed.
-
-  (* Lemma CompileTuples0_insert : *)
-  (*   forall vret vtable vtuple fpointer (env: Env ADTValue) ext tenv N idx *)
-  (*     (table: FiatBag N) (tuple: FiatTuple N), *)
-  (*     GLabelMap.find fpointer env = Some (Axiomatic Tuples0_insert) -> *)
-  (*     Lifted_MapsTo ext tenv vtable (wrap table) -> *)
-  (*     Lifted_MapsTo ext tenv vtuple (wrap tuple) -> *)
-  (*     Lifted_not_mapsto_adt ext tenv vret -> *)
-  (*     NoDuplicates [[[vret; vtable; vtuple]]] -> *)
-  (*     vret ∉ ext -> *)
-  (*     vtable ∉ ext -> *)
-  (*     vtuple ∉ ext -> *)
-  (*     BinNat.N.lt (BinNat.N.of_nat N) (Word.Npow2 32) -> *)
-  (*     minFreshIndex (IndexedEnsemble_TupleToListW table) idx -> *)
-  (*     {{ tenv }} *)
-  (*       Call vret fpointer (vtable :: vtuple :: nil) *)
-  (*     {{ [[ `vret <-- SCAZero as _ ]] *)
-  (*          :: [[ `vtable <-- table as _ ]] *)
-  (*          :: DropName vtable (DropName vret (DropName vtuple tenv)) }} ∪ {{ ext }} // env. *)
-  (* Proof. *)
-  (*   repeat (SameValues_Facade_t_step || facade_cleanup_call || LiftPropertyToTelescope_t || PreconditionSet_t). *)
-
-  (* Definition FiatBagFunctional {N} (fiatBag: FiatBag N) := *)
-  (*   forall t1 t2, *)
-  (*     fiatBag t1 -> fiatBag t2 -> *)
-  (*     IndexedEnsembles.elementIndex t1 = IndexedEnsembles.elementIndex t2 -> *)
-  (*     t1 = t2. *)
-
-  (* Definition FiatBagMinFreshIndex {N} (fiatBag: FiatBag N) idx := *)
-  (*   IndexedEnsembles.UnConstrFreshIdx fiatBag idx /\ *)
-  (*   (forall idx' : nat, (lt idx' idx) -> ~ IndexedEnsembles.UnConstrFreshIdx fiatBag idx'). *)
-
-  (* Record FiatBag' {N} := *)
-  (*   { fiatBag : FiatBag N; *)
-  (*     bagFunctional : FiatBagFunctional fiatBag; *)
-  (*     idx: nat; *)
-  (*     idxIsFresh: FiatBagMinFreshIndex fiatBag idx }. *)
-
-  (* Lemma minFreshIndex_Lift: *)
-  (*   forall (N : nat) (table : FiatBag N) (idx : nat), *)
-  (*     FiatBagMinFreshIndex table idx -> *)
-  (*     minFreshIndex (IndexedEnsemble_TupleToListW table) idx. *)
-  (* Proof. *)
-  (*   unfold FiatBagMinFreshIndex, minFreshIndex. *)
-  (*   repeat cleanup. *)
-
-  (*   Lemma UnconstrFreshIdx_Lift: *)
-  (*     forall (N : nat) (table : FiatBag N) (idx : nat), *)
-  (*       IndexedEnsembles.UnConstrFreshIdx table idx <-> UnConstrFreshIdx (IndexedEnsemble_TupleToListW table) idx. *)
-  (*   Proof. *)
-  (*     unfold IndexedEnsembles.UnConstrFreshIdx, UnConstrFreshIdx; *)
-  (*     repeat cleanup. *)
-  (*     rewrite <- IndexedElement_RoundTrip in H0. *)
-  (*     pose (IndexedEnsemble_TupleToListW_inj_helpe _ table (IndexedElement_ListWToTuple element)). H0). *)
-  (*   Admitted. *)
-
-  (*   apply UnconstrFreshIdx_Lift; assumption. *)
-  (*   rewrite <- UnconstrFreshIdx_Lift. *)
-  (*   eauto. *)
-  (* Qed. *)
-
-  (*   facade_eauto. *)
-  (*   facade_eauto. *)
-  (*   facade_eauto. *)
-  (*   admit. *)
-  (*   repeat apply DropName_remove; eauto 1. *)
-  (* Qed. *)
-
-  (* Lemma CompileTuples0_enumerate : *)
-  (*   forall vret vtable fpointer (env: Env ADTValue) ext tenv N *)
-  (*     (table: FiatBag N) (tuple: FiatTuple N), *)
-  (*     GLabelMap.find fpointer env = Some (Axiomatic Tuples0_enumerate) -> *)
-  (*     Lifted_MapsTo ext tenv vtable (wrap table) -> *)
-  (*     Lifted_not_mapsto_adt ext tenv vret -> *)
-  (*     NoDuplicates [[[vret; vtable]]] -> *)
-  (*     vret ∉ ext -> *)
-  (*     BinNat.N.lt (BinNat.N.of_nat N) (Word.Npow2 32) -> *)
-  (*     {{ tenv }} *)
-  (*       Call vret fpointer (vtable :: nil) *)
-  (*     {{ [[ `vret <-- @nil (FiatTuple N) as _ ]] :: DropName vret tenv }} ∪ {{ ext }} // env. *)
-  (* Proof. *)
-  (*   repeat (SameValues_Facade_t_step || facade_cleanup_call || LiftPropertyToTelescope_t || PreconditionSet_t). *)
-  (*   facade_eauto. *)
-  (*   admit.                      (* FIXME *) *)
-  (*   rewrite <- remove_add_comm by congruence. *)
-  (*   rewrite <- add_redundant_cancel by eassumption. *)
-  (*   facade_eauto. *)
-  (* Qed. *)
-End Tuples0.
-
-Section Tuples2.
-  Lemma CompileTuples2_new :
-    forall vret vsize vkey1 vkey2 fpointer (env: Env ADTValue) ext tenv N (k1 k2: W),
-      GLabelMap.find fpointer env = Some (Axiomatic Tuples2_new) ->
-      Lifted_MapsTo ext tenv vsize (wrap (Word.natToWord 32 N)) ->
-      Lifted_MapsTo ext tenv vkey1 (wrap k1) ->
-      Lifted_MapsTo ext tenv vkey2 (wrap k2) ->
-      Lifted_not_mapsto_adt ext tenv vret ->
-      vret ∉ ext ->
-      Word.wlt k1 (Word.natToWord 32 N) ->
-      Word.wlt k2 (Word.natToWord 32 N) ->
-      ~ Word.wlt (Word.natToWord 32 N) (Word.natToWord 32 2) ->
-      {{ tenv }}
-        Call vret fpointer (vsize :: vkey1 :: vkey2 :: nil)
-      {{ [[ (NTSome (H := @WrapInstance _ _ (QS_WrapBag2 k1 k2)) vret) <-- @FiatEmpty N as _ ]] :: DropName vret tenv }} ∪ {{ ext }} // env.
-  Proof.
-    repeat (SameValues_Facade_t_step || facade_cleanup_call || LiftPropertyToTelescope_t).
-    facade_eauto.
-    repeat f_equal; facade_eauto.
-    facade_eauto.
-  Qed.
-End Tuples2.
