src/CertifiedExtraction/Extraction/External/FacadeLoops.v
@@ -13,30 +13,6 @@ Ltac loop_unify_with_nil_t :=
 Ltac loop_t :=
   repeat (intros || unfold Fold || solve [PreconditionSet_t; Lifted_t] || compile_do_side_conditions || clean_DropName_in_ProgOk || rewrite Propagate_ret || eapply CompileSeq || eauto 2).
 
-Ltac apply_generalized_t compilation_lemma :=
-  erewrite ProgOk_TelEq_morphism;
-  try eapply compilation_lemma;
-  repeat match goal with
-         | [  |- _ = _ ] => reflexivity
-         | [  |- TelEq _ _ _ ] => decide_TelEq_instantiate
-         end.
-
-Tactic Notation "apply" "generalized" constr(compilation_lemma) :=
-  apply_generalized_t compilation_lemma.
-
-Ltac defunctionalize_evar :=
-  match goal with
-  | [  |- context[?e] ] =>
-    is_evar e;
-      match type of e with
-      | ?a -> ?b => let ee := fresh in
-                  evar (ee: b);
-                    unify e (fun _:a => ee);
-                    unfold ee in *;
-                    clear ee
-      end
-  end.
-
 Lemma CompileLoopBase :
   forall `{FacadeWrapper (Value av) A} `{FacadeWrapper (Value av) A'} `{FacadeWrapper av (list A)}
     lst init vhead vtest vlst vret fpop fempty fdealloc facadeBody env (ext: StringMap.t (Value av)) tenv (f: Comp A' -> A -> Comp A'),
