src/CertifiedExtraction/Extraction/Refactor/Basics.v
@@ -1,0 +1,33 @@
+Require Export Fiat.Computation.Notations.
+Require Export Fiat.ADT.Core Fiat.Computation.Core.
+Require Export Fiat.QueryStructure.Implementation.DataStructures.BagADT.QueryStructureImplementation.
+
+Require Export Bedrock.Platform.Facade.examples.TuplesF.
+Require Export CertifiedExtraction.Utils.
+Require Export Bedrock.Memory.
+
+Notation BedrockElement := (@TuplesF.IndexedElement (list W)).
+Notation BedrockBag := (@TuplesF.IndexedEnsemble (list W)).
+
+Fixpoint MakeVectorOfW N : Vector.t Type N :=
+  match N with
+  | O => Vector.nil Type
+  | S x => Vector.cons Type W x (MakeVectorOfW x)
+  end.
+
+Definition MakeWordHeading (N: nat) :=
+  {| NumAttr := N;
+     AttrList := MakeVectorOfW N |}.
+
+Notation FiatTuple N := (@RawTuple (MakeWordHeading N)).
+Notation FiatElement N := (@IndexedEnsembles.IndexedElement (FiatTuple N)).
+Notation FiatBag N := (@IndexedEnsembles.IndexedEnsemble (FiatTuple N)).
+
+Lemma MakeWordHeading_allWords :
+  forall {N} (idx: Fin.t N),
+    Domain (MakeWordHeading N) idx = W.
+Proof.
+  unfold MakeWordHeading; induction idx.
+  - reflexivity.
+  - unfold Domain in *; simpl in *; assumption.
+Defined.
