src/CertifiedExtraction/Extraction/Refactor/CallRules/Core.v
@@ -1,0 +1,43 @@
+Require Export Program.
+Require Export Fiat.Computation.Notations. (* FIXME remove *)
+Require Export Refactor.Basics.
+Require Export Refactor.TupleToListW.
+Require Export Refactor.EnsemblesOfTuplesAndListW.
+
+Require Export
+        Fiat.CertifiedExtraction.Extraction.External.Core
+        Fiat.CertifiedExtraction.Benchmarks.QueryStructureWrappers.
+
+Require Export Bedrock.Platform.Facade.examples.QsADTs.
+
+Ltac QS_t := match goal with
+             | |- not_mapsto_adt _ _ = true => eapply not_In_Telescope_not_in_Ext_not_mapsto_adt; eassumption
+             | _ => SameValues_Facade_t_step
+             | _ => facade_cleanup_call
+             | _ => LiftPropertyToTelescope_t
+             | _ => PreconditionSet_t
+             end.
+
+Ltac not_mapsto_adt_external_t :=
+  PreconditionSet_t;
+  repeat match goal with
+         | [ H: ?k <> ?s |- not_mapsto_adt ?k (StringMap.add ?s _ _) = true ] =>
+           apply not_mapsto_adt_neq_remove'; [ congruence | ]
+         | [ H: ?s <> ?k |- not_mapsto_adt ?k (StringMap.add ?s _ _) = true ] =>
+           apply not_mapsto_adt_neq_remove'; [ congruence | ]
+         | [  |- not_mapsto_adt ?k (StringMap.add ?k _ _) = true ] =>
+           apply not_mapsto_adt_eq_SCA
+         end.
+
+Ltac side_conditions_fast :=
+  repeat match goal with
+         | _ => apply CompileDeallocSCA_discretely; [ .. | apply ProgOk_Chomp_Some; intros ]
+         | |- NotInTelescope _ _ => simpl; repeat (split; intro; [ congruence | intros ]); eassumption
+         | [  |- _ ∉ _ ] => decide_not_in
+         end.
+
+Ltac fiat_t :=
+  repeat (eapply BindComputes || apply PickComputes || apply ReturnComputes || simpl).
+
+Hint Resolve Empty_lift : call_helpers_db.
+Hint Resolve TupleToListW_length : call_helpers_db.
