src/CertifiedExtraction/Extraction/Refactor/CallRules/Tuples0.v
@@ -1,0 +1,107 @@
+Require Export Fiat.Computation.Notations. (* FIXME remove *)
+Require Import Refactor.CallRules.Core.
+
+Lemma CompileTuples0_new :
+  forall vret vsize fpointer (env: Env ADTValue) ext tenv N,
+    GLabelMap.find fpointer env = Some (Axiomatic Tuples0_new) ->
+    Lifted_MapsTo ext tenv vsize (wrap (Word.natToWord 32 N)) ->
+    Lifted_not_mapsto_adt ext tenv vret ->
+    vret ∉ ext ->
+    ~ Word.wlt (Word.natToWord 32 N) (Word.natToWord 32 2) ->
+    {{ tenv }}
+      Call vret fpointer (vsize :: nil)
+    {{ [[ `vret <-- @FiatEmpty N as _ ]] :: DropName vret tenv }} ∪ {{ ext }} // env.
+Proof.
+  repeat (SameValues_Facade_t_step || facade_cleanup_call || LiftPropertyToTelescope_t).
+  facade_eauto.
+  repeat f_equal; facade_eauto. (* Uses Empty_lift *)
+  facade_eauto.
+Qed.
+
+(* Lemma CompileTuples0_insert : *)
+(*   forall vret vtable vtuple fpointer (env: Env ADTValue) ext tenv N idx *)
+(*     (table: FiatBag N) (tuple: FiatTuple N), *)
+(*     GLabelMap.find fpointer env = Some (Axiomatic Tuples0_insert) -> *)
+(*     Lifted_MapsTo ext tenv vtable (wrap table) -> *)
+(*     Lifted_MapsTo ext tenv vtuple (wrap tuple) -> *)
+(*     Lifted_not_mapsto_adt ext tenv vret -> *)
+(*     NoDuplicates [[[vret; vtable; vtuple]]] -> *)
+(*     vret ∉ ext -> *)
+(*     vtable ∉ ext -> *)
+(*     vtuple ∉ ext -> *)
+(*     BinNat.N.lt (BinNat.N.of_nat N) (Word.Npow2 32) -> *)
+(*     minFreshIndex (IndexedEnsemble_TupleToListW table) idx -> *)
+(*     {{ tenv }} *)
+(*       Call vret fpointer (vtable :: vtuple :: nil) *)
+(*     {{ [[ `vret <-- SCAZero as _ ]] *)
+(*          :: [[ `vtable <-- table as _ ]] *)
+(*          :: DropName vtable (DropName vret (DropName vtuple tenv)) }} ∪ {{ ext }} // env. *)
+(* Proof. *)
+(*   repeat (SameValues_Facade_t_step || facade_cleanup_call || LiftPropertyToTelescope_t || PreconditionSet_t). *)
+
+(* Definition FiatBagFunctional {N} (fiatBag: FiatBag N) := *)
+(*   forall t1 t2, *)
+(*     fiatBag t1 -> fiatBag t2 -> *)
+(*     IndexedEnsembles.elementIndex t1 = IndexedEnsembles.elementIndex t2 -> *)
+(*     t1 = t2. *)
+
+(* Definition FiatBagMinFreshIndex {N} (fiatBag: FiatBag N) idx := *)
+(*   IndexedEnsembles.UnConstrFreshIdx fiatBag idx /\ *)
+(*   (forall idx' : nat, (lt idx' idx) -> ~ IndexedEnsembles.UnConstrFreshIdx fiatBag idx'). *)
+
+(* Record FiatBag' {N} := *)
+(*   { fiatBag : FiatBag N; *)
+(*     bagFunctional : FiatBagFunctional fiatBag; *)
+(*     idx: nat; *)
+(*     idxIsFresh: FiatBagMinFreshIndex fiatBag idx }. *)
+
+(* Lemma minFreshIndex_Lift: *)
+(*   forall (N : nat) (table : FiatBag N) (idx : nat), *)
+(*     FiatBagMinFreshIndex table idx -> *)
+(*     minFreshIndex (IndexedEnsemble_TupleToListW table) idx. *)
+(* Proof. *)
+(*   unfold FiatBagMinFreshIndex, minFreshIndex. *)
+(*   repeat cleanup. *)
+
+(*   Lemma UnconstrFreshIdx_Lift: *)
+(*     forall (N : nat) (table : FiatBag N) (idx : nat), *)
+(*       IndexedEnsembles.UnConstrFreshIdx table idx <-> UnConstrFreshIdx (IndexedEnsemble_TupleToListW table) idx. *)
+(*   Proof. *)
+(*     unfold IndexedEnsembles.UnConstrFreshIdx, UnConstrFreshIdx; *)
+(*     repeat cleanup. *)
+(*     rewrite <- IndexedElement_RoundTrip in H0. *)
+(*     pose (IndexedEnsemble_TupleToListW_inj_helpe _ table (IndexedElement_ListWToTuple element)). H0). *)
+(*   Admitted. *)
+
+(*   apply UnconstrFreshIdx_Lift; assumption. *)
+(*   rewrite <- UnconstrFreshIdx_Lift. *)
+(*   eauto. *)
+(* Qed. *)
+
+(*   facade_eauto. *)
+(*   facade_eauto. *)
+(*   facade_eauto. *)
+(*   admit. *)
+(*   repeat apply DropName_remove; eauto 1. *)
+(* Qed. *)
+
+(* Lemma CompileTuples0_enumerate : *)
+(*   forall vret vtable fpointer (env: Env ADTValue) ext tenv N *)
+(*     (table: FiatBag N) (tuple: FiatTuple N), *)
+(*     GLabelMap.find fpointer env = Some (Axiomatic Tuples0_enumerate) -> *)
+(*     Lifted_MapsTo ext tenv vtable (wrap table) -> *)
+(*     Lifted_not_mapsto_adt ext tenv vret -> *)
+(*     NoDuplicates [[[vret; vtable]]] -> *)
+(*     vret ∉ ext -> *)
+(*     BinNat.N.lt (BinNat.N.of_nat N) (Word.Npow2 32) -> *)
+(*     {{ tenv }} *)
+(*       Call vret fpointer (vtable :: nil) *)
+(*     {{ [[ `vret <-- @nil (FiatTuple N) as _ ]] :: DropName vret tenv }} ∪ {{ ext }} // env. *)
+(* Proof. *)
+(*   repeat (SameValues_Facade_t_step || facade_cleanup_call || LiftPropertyToTelescope_t || PreconditionSet_t). *)
+(*   facade_eauto. *)
+(*   admit.                      (* FIXME *) *)
+(*   rewrite <- remove_add_comm by congruence. *)
+(*   rewrite <- add_redundant_cancel by eassumption. *)
+(*   facade_eauto. *)
+(* Qed. *)
