src/CertifiedExtraction/Extraction/Refactor/CallRules/Tuples2.v
@@ -1,0 +1,268 @@
+Require Export Fiat.Computation.Notations. (* FIXME remove *)
+Require Import Refactor.FiatBedrockLemmas.
+Require Import Refactor.CallRules.Core.
+
+Lemma CompileTuples2_new :
+  forall vret vsize vkey1 vkey2 fpointer (env: Env ADTValue) ext tenv N (k1 k2: W),
+    GLabelMap.find fpointer env = Some (Axiomatic Tuples2_new) ->
+    Lifted_MapsTo ext tenv vsize (wrap (Word.natToWord 32 N)) ->
+    Lifted_MapsTo ext tenv vkey1 (wrap k1) ->
+    Lifted_MapsTo ext tenv vkey2 (wrap k2) ->
+    Lifted_not_mapsto_adt ext tenv vret ->
+    vret ∉ ext ->
+    Word.wlt k1 (Word.natToWord 32 N) ->
+    Word.wlt k2 (Word.natToWord 32 N) ->
+    ~ Word.wlt (Word.natToWord 32 N) (Word.natToWord 32 2) ->
+    {{ tenv }}
+      Call vret fpointer (vsize :: vkey1 :: vkey2 :: nil)
+    {{ [[ (NTSome (H := @WrapInstance _ _ (QS_WrapBag2 k1 k2)) vret) <-- @FiatEmpty N as _ ]] :: DropName vret tenv }} ∪ {{ ext }} // env.
+Proof.
+  repeat (SameValues_Facade_t_step || facade_cleanup_call || LiftPropertyToTelescope_t).
+  facade_eauto.
+  repeat f_equal; facade_eauto.
+  facade_eauto.
+Qed.
+
+Lemma CompileTuples2_findFirst :
+  forall vret vtable vkey fpointer (env: Env QsADTs.ADTValue) ext tenv N (idx1 : Fin.t N)
+         (k1 := (Word.natToWord 32 (projT1 (Fin.to_nat idx1)))) k2
+         (table: FiatBag N) (key: W)
+         (table':= ( results <- {l : list RawTuple |
+                                 IndexedEnsembles.EnsembleIndexedListEquivalence
+                                   (IndexedEnsembles.IndexedEnsemble_Intersection
+                                      (table)
+                                      (fun x0 : RawTuple =>
+                                         ((if Word.weq match MakeWordHeading_allWords idx1 in _ = W return W with
+                                                       | eq_refl => GetAttributeRaw x0 idx1
+                                                       end key then true else false) && true)%bool = true)) l};
+                     ret (table, results))
+                   : Comp (_ * list (FiatTuple N))),
+    GLabelMap.MapsTo fpointer (Axiomatic QsADTs.Tuples2_findFirst) env ->
+    Lifted_MapsTo ext tenv vtable (wrap (FacadeWrapper := @WrapInstance _ _ (QS_WrapBag2 k1 k2)) table) ->
+    Lifted_MapsTo ext tenv vkey (wrap key) ->
+    Lifted_not_mapsto_adt ext tenv vret ->
+    NoDuplicates [[[vret; vtable; vkey]]] ->
+    vret ∉ ext ->
+    vtable ∉ ext ->
+    (* IndexedEnsembles.UnConstrFreshIdx table idx -> *)
+    BinNat.N.lt (BinNat.N.of_nat N) (Word.Npow2 32) ->
+    TuplesF.functional (IndexedEnsemble_TupleToListW table) ->
+    {{ tenv }}
+      Call vret fpointer (vtable :: vkey :: nil)
+    {{ [[ table' as retv ]]
+           :: [[ (@NTSome QsADTs.ADTValue _ vtable (@WrapInstance _ _ (QS_WrapBag2 k1 k2))) <-- fst retv as _ ]]
+           :: [[ (@NTSome QsADTs.ADTValue _ vret (@WrapInstance _ _ QS_WrapTupleList)) <-- snd retv as _ ]]
+           :: DropName vret (DropName vtable tenv) }} ∪ {{ ext }} // env.
+Proof.
+  repeat (SameValues_Facade_t_step || facade_cleanup_call || LiftPropertyToTelescope_t || PreconditionSet_t).
+
+  fiat_t.
+  5:solve[repeat apply DropName_remove; eauto 1].
+  4:solve[simpl; eauto using f_equal, ListWToTuple_Truncated_map_keepEq].
+  3:solve[fiat_t].
+  2:solve[fiat_t].
+
+  wipe.
+
+  apply Fiat_Bedrock_Filters_Equivalence; assumption.
+Qed.
+
+Print Assumptions CompileTuples2_findFirst.
+
+Lemma CompileTuples2_findFirst_spec :
+  forall vret vtable vkey fpointer (env: Env QsADTs.ADTValue) ext tenv N
+         (idx1 : Fin.t N)
+         (k1 := (Word.natToWord 32 (projT1 (Fin.to_nat idx1))))
+         k2
+         (table: FiatBag N) (key: W)
+         (table':= ( results <- {l : list RawTuple |
+                                 IndexedEnsembles.EnsembleIndexedListEquivalence
+                                   (IndexedEnsembles.IndexedEnsemble_Intersection
+                                      (table)
+                                      (fun x0 : RawTuple =>
+                                         ((if Word.weq match MakeWordHeading_allWords idx1 in _ = W return W with
+                                                       | eq_refl => GetAttributeRaw x0 idx1
+                                                       end key then true else false) && true)%bool = true)) l};
+                     ret (table, results))
+                   : Comp (_ * list (FiatTuple N))),
+    BinNat.N.lt (BinNat.N.of_nat N) (Word.Npow2 32) ->
+    GLabelMap.MapsTo fpointer (Axiomatic QsADTs.Tuples2_findFirst) env ->
+    StringMap.MapsTo vkey (wrap key) ext ->
+    PreconditionSet tenv ext [[[vret; vtable]]] ->
+    vret <> vkey ->
+    vtable <> vkey ->
+    TuplesF.functional (IndexedEnsemble_TupleToListW table) ->
+    {{ [[ (@NTSome QsADTs.ADTValue _ vtable (@WrapInstance _ _ (QS_WrapBag2 k1 k2))) <-- table as _]] :: tenv }}
+      Call vret fpointer (vtable :: vkey :: nil)
+    {{ [[ table' as retv ]]
+           :: [[ (@NTSome QsADTs.ADTValue _ vtable (@WrapInstance _ _ (QS_WrapBag2 k1 k2))) <-- fst retv as _ ]]
+           :: [[ (@NTSome QsADTs.ADTValue _ vret (@WrapInstance _ _ QS_WrapTupleList)) <-- snd retv as _ ]]
+           :: tenv }} ∪ {{ ext }} // env.
+Proof.
+  intros.
+  apply generalized CompileTuples2_findFirst; repeat (compile_do_side_conditions || Lifted_t || PreconditionSet_t).
+  setoid_rewrite (DropName_NotInTelescope _ _ H12).
+  rewrite DropName_Cons_None.
+  setoid_rewrite (DropName_NotInTelescope _ _ H10).
+  decide_TelEq_instantiate.
+Qed.
+
+Lemma CompileTuples2_insert :
+  forall vret vtable vtuple fpointer (env: Env QsADTs.ADTValue) ext tenv N k1 k2 idx
+    (table: FiatBag N) (tuple: FiatTuple N),
+    GLabelMap.MapsTo fpointer (Axiomatic QsADTs.Tuples2_insert) env ->
+    Lifted_MapsTo ext tenv vtable (wrap (FacadeWrapper := @WrapInstance _ _ (QS_WrapBag2 k1 k2)) table) ->
+    Lifted_MapsTo ext tenv vtuple (wrap tuple) ->
+    Lifted_not_mapsto_adt ext tenv vret ->
+    NoDuplicates [[[vret; vtable; vtuple]]] ->
+    vret ∉ ext ->
+    vtable ∉ ext ->
+    vtuple ∉ ext ->
+    BinNat.N.lt (BinNat.N.of_nat N) (Word.Npow2 32) ->
+    TuplesF.minFreshIndex (IndexedEnsemble_TupleToListW table) idx ->
+    {{ tenv }}
+      Call vret fpointer (vtable :: vtuple :: nil)
+    {{ [[ ( freshIdx <- {freshIdx : nat | IndexedEnsembles.UnConstrFreshIdx table freshIdx};
+                ret (Ensembles.Add IndexedEnsembles.IndexedElement table
+                                   {| IndexedEnsembles.elementIndex := freshIdx;
+                                      IndexedEnsembles.indexedElement := tuple |})) as rep ]]
+           :: [[`vret <-- (Word.natToWord 32 0) as _ ]]
+           :: [[ (NTSome (H := @WrapInstance _ _ (QS_WrapBag2 k1 k2)) vtable) <-- rep as _ ]]
+           :: DropName vtable (DropName vret (DropName vtuple tenv)) }} ∪ {{ ext }} // env.
+Proof.
+  repeat (SameValues_Facade_t_step || facade_cleanup_call || LiftPropertyToTelescope_t || PreconditionSet_t).
+  facade_eauto.
+  fiat_t.
+  apply minFresh_UnConstrFresh; eauto.
+  facade_eauto.
+  facade_eauto.
+
+  repeat f_equal.
+  apply Ensembles.Extensionality_Ensembles.
+
+  lazymatch goal with
+  | [ H: TuplesF.minFreshIndex _ ?x, H': TuplesF.minFreshIndex _ ?y |- _ ] =>
+    learn (minFreshIndex_unique H H'); subst
+  end.
+
+  apply Fiat_Bedrock_Insert.
+  repeat apply DropName_remove; eauto 1.
+Qed.
+
+Lemma CompileTuples2_insert_spec :
+  forall vtmp vtable vtuple fpointer (env: Env QsADTs.ADTValue) ext tenv N k1 k2 idx
+    (table: FiatBag N) (tuple: FiatTuple N),
+    GLabelMap.MapsTo fpointer (Axiomatic QsADTs.Tuples2_insert) env ->
+    NoDuplicates [[[vtmp; vtable; vtuple]]] ->
+    vtmp ∉ ext ->
+    vtable ∉ ext ->
+    vtuple ∉ ext ->
+    NotInTelescope vtmp tenv ->
+    NotInTelescope vtuple tenv ->
+    NotInTelescope vtable tenv ->
+    BinNat.N.lt (BinNat.N.of_nat N) (Word.Npow2 32) ->
+    TuplesF.minFreshIndex (IndexedEnsemble_TupleToListW table) idx ->
+    {{ [[ (NTSome (H := @WrapInstance _ _ (QS_WrapBag2 k1 k2)) vtable) <-- table as _ ]]
+         :: [[ (NTSome (H := @WrapInstance _ _ QS_WrapTuple) vtuple) <-- tuple as _ ]]
+         :: tenv }}
+      Call vtmp fpointer (vtable :: vtuple :: nil)
+    {{ [[ ( freshIdx <- {freshIdx : nat | IndexedEnsembles.UnConstrFreshIdx table freshIdx};
+                ret (Ensembles.Add IndexedEnsembles.IndexedElement table
+                                   {| IndexedEnsembles.elementIndex := freshIdx;
+                                      IndexedEnsembles.indexedElement := tuple |})) as rep ]]
+           :: [[ (NTSome (H := @WrapInstance _ _ (QS_WrapBag2 k1 k2)) vtable) <-- rep as _ ]]
+           :: tenv }} ∪ {{ ext }} // env.
+Proof.
+  intros. PreconditionSet_t.
+  apply ProgOk_Remove_Skip_R; hoare.
+  apply generalized CompileTuples2_insert; repeat (compile_do_side_conditions || Lifted_t).
+  eauto.
+  apply ProgOk_Chomp_None; intros.
+  repeat match goal with
+         | [ H: NotInTelescope ?k ?tenv |- context[DropName ?k ?tenv] ] => setoid_rewrite (DropName_NotInTelescope _ _ H)
+         | _ => setoid_rewrite Propagate_anonymous_ret
+         | _ => fold @DropName
+         end.
+  apply CompileDeallocSCA_discretely; repeat (compile_do_side_conditions || decide_NotInTelescope).
+  apply CompileSkip.
+Qed.
+
+
+Lemma CompileTuples2_findSecond :
+  forall vret vtable vkey fpointer (env: Env QsADTs.ADTValue) ext tenv N k1
+    (table: FiatBag N) (key: W) (idx2: Fin.t N)
+    (k2 := (Word.natToWord 32 (projT1 (Fin.to_nat idx2))))
+    (table':= ( results <- {l : list RawTuple |
+                          IndexedEnsembles.EnsembleIndexedListEquivalence
+                            (IndexedEnsembles.IndexedEnsemble_Intersection
+                               table
+                               (fun x0 : RawTuple =>
+                                  ((if Word.weq match MakeWordHeading_allWords idx2 in _ = W return W with
+                                                | eq_refl => GetAttributeRaw x0 idx2
+                                                end key then true else false) && true)%bool =
+                                  true)) l};
+                 ret (table, results))%comp
+             : Comp (_ * list (FiatTuple N))),
+    GLabelMap.MapsTo fpointer (Axiomatic QsADTs.Tuples2_findSecond) env ->
+    Lifted_MapsTo ext tenv vtable (wrap (FacadeWrapper := @WrapInstance _ _ (QS_WrapBag2 k1 k2)) table) ->
+    Lifted_MapsTo ext tenv vkey (wrap key) ->
+    Lifted_not_mapsto_adt ext tenv vret ->
+    NoDuplicates [[[vret; vtable; vkey]]] ->
+    vret ∉ ext ->
+    vtable ∉ ext ->
+    BinNat.N.lt (BinNat.N.of_nat N) (Word.Npow2 32) ->
+    TuplesF.functional (IndexedEnsemble_TupleToListW table) ->
+    {{ tenv }}
+      Call vret fpointer (vtable :: vkey :: nil)
+    {{ [[ table' as retv ]]
+           :: [[ (@NTSome QsADTs.ADTValue _ vtable (@WrapInstance _ _ (QS_WrapBag2 k1 k2))) <-- fst retv as _ ]]
+           :: [[ (@NTSome QsADTs.ADTValue _ vret (@WrapInstance _ _ QS_WrapTupleList)) <-- snd retv as _ ]]
+           :: DropName vret (DropName vtable tenv) }} ∪ {{ ext }} // env.
+Proof.
+  repeat (SameValues_Facade_t_step || facade_cleanup_call || LiftPropertyToTelescope_t || PreconditionSet_t).
+  fiat_t.
+
+  5:solve[repeat apply DropName_remove; eauto 1].
+  4:solve[simpl; eauto using f_equal, ListWToTuple_Truncated_map_keepEq].
+  3:solve[fiat_t].
+  2:solve[fiat_t].
+
+  apply Fiat_Bedrock_Filters_Equivalence; eassumption.
+Qed.
+
+Lemma CompileTuples2_findSecond_spec :
+  forall vret vtable vkey fpointer (env: Env QsADTs.ADTValue) ext tenv N k1
+    (table: FiatBag N) (key: W) (idx2: Fin.t N)
+    (k2 := (Word.natToWord 32 (projT1 (Fin.to_nat idx2))))
+    (table':= ( results <- {l : list RawTuple |
+                          IndexedEnsembles.EnsembleIndexedListEquivalence
+                            (IndexedEnsembles.IndexedEnsemble_Intersection
+                               table
+                               (fun x0 : RawTuple =>
+                                  ((if Word.weq match MakeWordHeading_allWords idx2 in _ = W return W with
+                                                | eq_refl => GetAttributeRaw x0 idx2
+                                                end key then true else false) && true)%bool =
+                                  true)) l};
+                 ret (table, results))%comp
+             : Comp (_ * list (FiatTuple N))),
+    GLabelMap.MapsTo fpointer (Axiomatic QsADTs.Tuples2_findSecond) env ->
+    StringMap.MapsTo vkey (wrap key) ext ->
+    PreconditionSet tenv ext [[[vret; vtable]]] ->
+    vret <> vkey ->
+    vtable <> vkey ->
+    BinNat.N.lt (BinNat.N.of_nat N) (Word.Npow2 32) ->
+    TuplesF.functional (IndexedEnsemble_TupleToListW table) ->
+    {{ [[ (@NTSome QsADTs.ADTValue _ vtable (@WrapInstance _ _ (QS_WrapBag2 k1 k2))) <-- table as _]] :: tenv }}
+      Call vret fpointer (vtable :: vkey :: nil)
+    {{ [[ table' as retv ]]
+         :: [[ (@NTSome QsADTs.ADTValue _ vtable (@WrapInstance _ _ (QS_WrapBag2 k1 k2))) <-- fst retv as _ ]]
+         :: [[ (@NTSome QsADTs.ADTValue _ vret (@WrapInstance _ _ QS_WrapTupleList)) <-- snd retv as _ ]]
+         :: tenv }} ∪ {{ ext }} // env.
+Proof.
+  intros.
+  apply generalized CompileTuples2_findSecond; repeat (compile_do_side_conditions || Lifted_t || PreconditionSet_t).
+  setoid_rewrite (DropName_NotInTelescope _ _ H12).
+  rewrite DropName_Cons_None.
+  setoid_rewrite (DropName_NotInTelescope _ _ H10).
+  decide_TelEq_instantiate.
+Qed.
