src/CertifiedExtraction/Extraction/Refactor/QueryStructureWrappersAreConsistent.v
@@ -1,0 +1,40 @@
+Require Import Fiat.CertifiedExtraction.Benchmarks.QueryStructureWrappers.
+Require Import Fiat.CertifiedExtraction.ADT2CompileUnit.
+Require Import CertifiedExtraction.Core.
+Require Import Bedrock.Memory.
+Require Import FacadeUtils.
+
+
+(* FIXME: Just embed the definition of ‘Good’ into the ‘Wrapper’ typeclass *)
+
+Definition Good_bool {av}
+  : GoodWrapper av bool.
+Proof.
+  refine {| gWrap := _;
+            gWrapTag := false |}; simpl; eauto.
+Defined.
+
+Definition Good_listW
+  : GoodWrapper QsADTs.ADTValue (list W).
+Proof.
+  refine {| gWrap := WrapInstance (H := QS_WrapWordList);
+            gWrapTag := true |};
+    simpl; eauto.
+Defined.
+
+Definition Good_BedrockTuple
+  : GoodWrapper QsADTs.ADTValue (list W).
+Proof.
+  refine {| gWrap := WrapInstance (H := QS_WrapBedrockTuple);
+            gWrapTag := true
+         |}; intros; unfold wrap; simpl; eauto.
+Defined.
+
+Definition Good_W {av}
+  : GoodWrapper av W.
+Proof.
+  refine {| gWrap := _;
+            gWrapTag := false
+         |}; intros; unfold wrap; simpl; eauto.
+Defined.
+
